work on heap modeling with @nik

ulib/FStar.Array.fst
@@ -27,9 +27,9 @@ assume val op_At_Bar: #a:Type -> array a -> array a -> St (array a)
 
 assume val of_seq: #a:Type -> s:seq a -> ST (array a)
   (requires (fun h -> True))
-  (ensures  (fun h0 x h1 -> (not(contains h0 x)
+  (ensures  (fun h0 x h1 -> (~ (contains h0 x)
                              /\ contains h1 x
-                             /\ modifies TSet.empty h0 h1
+                             /\ modifies Set.empty h0 h1
                              /\ sel h1 x==s)))
 
 assume val to_seq: #a:Type -> s:array a -> ST (seq a)
@@ -38,10 +38,14 @@ assume val to_seq: #a:Type -> s:array a -> ST (seq a)
 
 assume val create : #a:Type -> n:nat -> init:a -> ST (array a)
   (requires (fun h -> True))
-  (ensures  (fun h0 x h1 -> (not(contains h0 x)
+  (ensures  (fun h0 x h1 -> (~ (contains h0 x)
                              /\ contains h1 x
-                             /\ modifies TSet.empty h0 h1
+                             /\ modifies Set.empty h0 h1
                              /\ sel h1 x==Seq.create n init)))
+  (* (ensures  (fun h0 x h1 -> (~ (contains h0 x) *)
+  (*                            /\ contains h1 x *)
+  (*                            /\ modifies Set.empty h0 h1 *)
+  (*                            /\ sel h1 x==Seq.create n init))) *)
 
 assume val index : #a:Type -> x:array a -> n:nat -> ST a
   (requires (fun h -> contains h x /\ n < Seq.length (sel h x)))
@@ -62,34 +66,37 @@ assume val length: #a:Type -> x:array a -> ST nat
 
 assume val op: #a:Type -> f:(seq a -> Tot (seq a)) -> x:array a -> ST unit
   (requires (fun h -> contains h x))
-  (ensures  (fun h0 u h1 -> modifies (TSet.singleton (Ref x)) h0 h1 /\ sel h1 x==f (sel h0 x)))
+  (ensures  (fun h0 u h1 -> modifies (only x) h0 h1 /\ sel h1 x==f (sel h0 x)))
 
 val swap: #a:Type -> x:array a -> i:nat -> j:nat{i <= j}
                  -> ST unit (requires (fun h -> contains h x /\ j < Seq.length (sel h x)))
                             (ensures (fun h0 _u h1 ->
                                       (j < Seq.length (sel h0 x))
                                       /\ contains h1 x
-                                      /\ (h1==Heap.upd h0 x (SeqProperties.swap (sel h0 x) i j))))
+				      /\ modifies (only x) h0 h1))
+				      (* /\ sel h1 x == SeqProperties.swap (sel h0 x) i j)) *)
+                                      (* /\ (h1==Heap.upd h0 x (SeqProperties.swap (sel h0 x) i j)))) *)
 let swap #a x i j =
   let h0 = get () in
   let tmpi = index x i in
   let tmpj = index x j in
   upd x j tmpi;
   upd x i tmpj;
-  let h1 = get () in
-  let s1 = sel h1 x in
-  cut (b2t(equal h1 (Heap.upd h0 x s1)))
+  //let h1 = get () in
+  //let s1 = sel h1 x in
+  ()
+  //cut (b2t(equal h1 (Heap.upd h0 x s1)))
 
 (* Helper functions for stateful array manipulation *)
 val copy_aux:
   #a:Type -> s:array a -> cpy:array a -> ctr:nat ->
      ST unit
-	(requires (fun h -> (contains h s /\ contains h cpy /\ s =!= cpy)
+	(requires (fun h -> (contains h s /\ contains h cpy /\ addr_of s <> addr_of cpy)
 			    /\ (Seq.length (sel h cpy) = Seq.length (sel h s))
 			    /\ (ctr <= Seq.length (sel h cpy))
 			    /\ (forall (i:nat). i < ctr ==> Seq.index (sel h s) i == Seq.index (sel h cpy) i)))
-	(ensures (fun h0 u h1 -> (contains h1 s /\ contains h1 cpy /\ s =!= cpy )
-			      /\ (modifies (TSet.singleton (Ref cpy)) h0 h1)
+	(ensures (fun h0 u h1 -> (contains h1 s /\ contains h1 cpy /\ addr_of s <> addr_of cpy )
+			      /\ (modifies (only cpy) h0 h1)
 			      /\ (Seq.equal (sel h1 cpy) (sel h1 s))))
 let rec copy_aux #a s cpy ctr =
   match length cpy - ctr with
@@ -102,8 +109,8 @@ val copy:
   ST (array a)
      (requires (fun h -> contains h s
 			 /\ Seq.length (sel h s) > 0))
-     (ensures (fun h0 r h1 -> (modifies TSet.empty h0 h1)
-				     /\ not(contains h0 r)
+     (ensures (fun h0 r h1 -> (modifies Set.empty h0 h1)
+				     /\ ~ (contains h0 r)
 				     /\ (contains h1 r)
 				     /\ (Seq.equal (sel h1 r) (sel h0 s))))
 let copy #a s =
@@ -115,15 +122,15 @@ val blit_aux:
   #a:Type -> s:array a -> s_idx:nat -> t:array a -> t_idx:nat -> len:nat -> ctr:nat ->
   ST unit
      (requires (fun h ->
-		(contains h s /\ contains h t /\ s =!= t)
+		(contains h s /\ contains h t /\ addr_of s <> addr_of t)
 		/\ (Seq.length (sel h s) >= s_idx + len)
 		/\ (Seq.length (sel h t) >= t_idx + len)
 		/\ (ctr <= len)
 		/\ (forall (i:nat).
 		    i < ctr ==> Seq.index (sel h s) (s_idx+i) == Seq.index (sel h t) (t_idx+i))))
      (ensures (fun h0 u h1 ->
-	       (contains h1 s /\ contains h1 t /\ s =!= t )
-	       /\ (modifies (TSet.singleton (Ref t)) h0 h1)
+	       (contains h1 s /\ contains h1 t /\ addr_of s <> addr_of t)
+	       /\ (modifies (only t) h0 h1)
 	       /\ (Seq.length (sel h1 s) >= s_idx + len)
 	       /\ (Seq.length (sel h1 t) >= t_idx + len)
 	       /\ (Seq.length (sel h0 s) = Seq.length (sel h1 s))
@@ -145,16 +152,16 @@ val blit:
      (requires (fun h ->
 		(contains h s)
 		/\ (contains h t)
-		/\ (s =!= t)
+		/\ (addr_of s <> addr_of t)
 		/\ (Seq.length (sel h s) >= s_idx + len)
 		/\ (Seq.length (sel h t) >= t_idx + len)))
      (ensures (fun h0 u h1 ->
-	       (contains h1 s /\ contains h1 t /\ s =!= t )
+	       (contains h1 s /\ contains h1 t /\ addr_of s <> addr_of t)
 	       /\ (Seq.length (sel h1 s) >= s_idx + len)
 	       /\ (Seq.length (sel h1 t) >= t_idx + len)
 	       /\ (Seq.length (sel h0 s) = Seq.length (sel h1 s))
 	       /\ (Seq.length (sel h0 t) = Seq.length (sel h1 t))
-	       /\ (modifies (TSet.singleton (Ref t)) h0 h1)
+	       /\ (modifies (only t) h0 h1)
 	       /\ (forall (i:nat).
 		   i < len ==> Seq.index (sel h1 s) (s_idx+i) == Seq.index (sel h1 t) (t_idx+i))
 	       /\ (forall (i:nat).
@@ -173,8 +180,8 @@ val sub :
     (ensures (fun h0 t h1 ->
       (contains h1 t)
       /\ (contains h0 s)
-      /\ not(contains h0 t)
-      /\ (modifies (TSet.empty) h0 h1)
+      /\ ~ (contains h0 t)
+      /\ (modifies Set.empty h0 h1)
       /\ (Seq.length (sel h0 s) > 0)
       /\ (idx + len <= Seq.length (sel h0 s))
       /\ (Seq.equal (Seq.slice (sel h0 s) idx (idx+len)) (sel h1 t))))
@@ -182,3 +189,6 @@ let sub #a s idx len =
   let t = create len (index s 0) in
   blit s idx t 0 len;
   t
+
+val foo: n:nat -> St nat (decreases n)
+let rec foo n = foo (n + 1)
